ADTRefinement.v
@@ -30,7 +30,6 @@ Section pick.
   Program Definition pickImpl : ADT :=
     {|
       Rep := rep;
-      RepInv m := True;
       MutatorIndex := mutatorMethodIndex;
       ObserverIndex := observerMethodIndex;
       MutatorMethods idx :=
@@ -49,23 +48,25 @@ Section MethodRefinement.
   Variables oldRep newRep : Type.
   (** Old and new representations **)
 
-  Variable oldRepInv : Ensemble oldRep.
-  Variable newRepInv : Ensemble newRep.
-  (** Old and new representation invariants **)
+  Variable BiR : oldRep -> newRep -> Prop.
+  (** Bisimulation Relation *)
 
-  Variable abs : newRep -> Comp oldRep.
-  (** Abstraction function *)
+  Notation "ro ≃ rn" := (BiR ro rn) (at level 70).
 
-  (** Refinement of a mutator method: if we first do the new
-      computation and then abstract, this is a refinement of first
-      abstracting and then doing the old computation.  That is, the
+  (** Refinement of a mutator method: the values of the computation
+      produced by applying a new mutator method [newMutator] to any new
+      state [r_n] related to an old state [r_o] by the bisimulation
+      relation [BiR] are related by [BiR] to some value produced by
+      the corresponding old mutator on [r_o]. Related values
+      are taken to related values (with the new mutator potentially
+      producing more deterministic computations). That is, the
       following diagram commutes:
 <<
                    old mutator
        old rep --------------> old rep
-          ↑                         ↑
-      abs |                         | abs
           |                         |
+      BiR |                         | BiR
+          ↓                         ↓
        new rep --------------> new rep
                    new mutator
 >>  *)
@@ -73,94 +74,71 @@ Section MethodRefinement.
   Definition refineMutator
              (oldMutator : mutatorMethodType oldRep)
              (newMutator : mutatorMethodType newRep)
-    := forall new_state n,
-         newRepInv new_state ->
-         refine (old_state <- abs new_state;
-                 oldMutator old_state n)
-                (new_state' <- newMutator new_state n;
-                 abs new_state').
+    := forall r_o r_n n, r_o ≃ r_n ->
+         refine (r_o' <- oldMutator r_o n;
+                 {r_n | r_o' ≃ r_n})
+                (newMutator r_n n).
 
-  (** Refinement of an observer method: the new computation should be
-      a refinement of first abstracting and then doing the old
-      computation.  That is, the following diagram should commute:
+  (** Refinement of an observer method: the computation produced by
+   an observer [newObserver] on any new state [r_n] related to an old
+   state [r_o] by the bisimulation relation [BiR] should be a refinement
+   of the computation produced by the old observer [oldObserver] on
+   [r_n].  That is, the following diagram should commute:
 <<
                   old observer
        old rep --------------> ℕ
-          ↑                      ∥
-      abs |                      ∥ id
           |                      ∥
+      BiR |                      ∥ id
+          ↓                      ∥
        new rep --------------> ℕ
                   new observer
 >>
    *)
+
   Definition refineObserver
              (oldObserver : observerMethodType oldRep)
              (newObserver : observerMethodType newRep)
-    := forall new_state n,
-         newRepInv new_state ->
-         refine (old_state <- abs new_state;
-                 oldObserver old_state n)
-                (newObserver new_state n).
-
-  (**  Abstraction should preserve representation invariants:
-       The abstraction of a new representation that satisfies its
-       representation invariant should satisfy the old invariant.
-       Diagrammatically,
-
-  (Old RepInv holds)
-      old rep
-        ↑
-        | abs
-        |
-       new rep
-  (New RepInv holds)
-   **)
-
-  Definition absPreservesInv
-    := forall new_state,
-         newRepInv new_state ->
-         computational_inv oldRepInv (abs new_state).
+    := forall r_o r_n n, r_o ≃ r_n ->
+         refine (oldObserver r_o n)
+                (newObserver r_n n).
 
 End MethodRefinement.
+
+  Notation "c ↝ v" := (computes_to c v) (at level 70).
 
 (** We map from old indices to new indices because every method that
     used to be callable should still be callable, and we don't care
     about the other methods. *)
 Inductive refineADT (A B : ADT) : Prop :=
 | refinesADT :
-    forall abs mutatorMap observerMap,
+    forall BiR mutatorMap observerMap,
       (forall idx, @refineMutator
                      (Rep A) (Rep B)
-                     (RepInv B) abs
+                     BiR
                      (MutatorMethods A idx)
                      (MutatorMethods B (mutatorMap idx)))
       -> (forall idx, @refineObserver
                      (Rep A) (Rep B)
-                     (RepInv B) abs
+                     BiR
                      (ObserverMethods A idx)
                      (ObserverMethods B (observerMap idx)))
-      -> (@absPreservesInv (Rep A) (Rep B)
-                 (RepInv A) (RepInv B) abs)
       -> refineADT A B.
 
 (** We should always just unfold [refineMutator] and [refineObserver]
     into [refine], so that we can rewrite with lemmas about [refine]. *)
 Arguments refineMutator / .
 Arguments refineObserver / .
-Arguments absPreservesInv / .
 
-Instance refineMutator_refl rep repInv
-: Reflexive (@refineMutator rep rep repInv (@Return _)).
+Instance refineMutator_refl rep
+: Reflexive (@refineMutator rep rep eq).
 Proof.
-  intro; simpl; intros.
-  autorewrite with refine_monad; reflexivity.
+  intro; simpl; intros; subst; econstructor; eauto.
 Qed.
 
-Instance refineObserver_refl rep repInv
-: Reflexive (@refineObserver rep rep repInv (@Return _)).
+Instance refineObserver_refl rep
+: Reflexive (@refineObserver rep rep eq).
 Proof.
-  intro; simpl; intros.
-  autorewrite with refine_monad; reflexivity.
+  intro; simpl; intros; subst; reflexivity.
 Qed.
 
 Global Instance refineADT_PreOrder : PreOrder refineADT.
@@ -168,32 +146,24 @@ Proof.
   split; compute in *.
   - intro x.
     econstructor 1 with
-    (abs := @Return _)
+    (BiR := eq)
       (mutatorMap := id)
       (observerMap := id);
       unfold id;
       try reflexivity.
-    simpl; intros;
-      inversion_by computes_to_inv; subst; eauto.
   - intros x y z
-           [abs mutMap obsMap mutH obsH]
-           [abs' mutMap' obsMap' mutH' obsH'].
+           [BiR mutMap obsMap mutH obsH]
+           [BiR' mutMap' obsMap' mutH' obsH'].
     econstructor 1 with
-      (abs := fun z => (z' <- abs' z; abs z')%comp)
+      (BiR := fun x z => exists y, BiR x y /\ BiR' y z)
         (mutatorMap := mutMap' ∘ mutMap)
         (observerMap := obsMap' ∘ obsMap);
     unfold id, compose; simpl in *; intros.
-    + autorewrite with refine_monad.
-      rewrite <- !refineEquiv_bind_bind, <- mutH', !refineEquiv_bind_bind; eauto.
-      unfold refine; intros; inversion_by computes_to_inv.
+    + destruct_ex; intuition.
+      rewrite <- mutH', <- mutH; eauto.
+      intros r_n' Comp_n'; inversion_by computes_to_inv.
       econstructor; eauto.
-      eapply mutH; eauto.
-    + autorewrite with refine_monad.
-      rewrite <- !refineEquiv_bind_bind, <- obsH', refineEquiv_bind_bind; eauto.
-      unfold refine; intros; inversion_by computes_to_inv.
-      econstructor; eauto.
-      eapply obsH; eauto.
-    + inversion_by computes_to_inv; eauto.
+    + destruct_ex; intuition; rewrite obsH, obsH'; eauto; reflexivity.
 Qed.
 
 Add Parametric Relation : ADT refineADT
@@ -238,118 +208,10 @@ Add Parametric Relation : ADT refineADT
 
 Section GeneralRefinements.
 
-  (* Refining Observers is a valid ADT refinement. *)
-  Add Parametric Morphism rep repInv mutIdx obsIdx ms mutInv
-  : (fun os => @Build_ADT rep repInv mutIdx obsIdx ms os mutInv)
-    with signature
-    (pointwise_relation _ (@refineObserver _ _ repInv (@Return _)))
-      ==> refineADT
-      as refineADT_Build_ADT_Observer.
-  Proof.
-    intros.
-    let A := match goal with |- refineADT ?A ?B => constr:(A) end in
-    let B := match goal with |- refineADT ?A ?B => constr:(B) end in
-    eapply (@refinesADT A B (@Return _) id id);
-      unfold id, pointwise_relation in *; simpl in *; intros;
-      auto; try inversion_by computes_to_inv; subst; eauto;
-      autorewrite with refine_monad; reflexivity.
-  Qed.
+  (* Refining the representation type is a valid refinement,
+     as long as the new methods are valid refinements.
 
-  (* Refining Mutators is also a valid ADT refinement, but it's
-   harder to express as a morphism because of the dependence of
-   [MutatorMethodsInv] on [MutatorMethods]. *)
-
-  Lemma refineMutatorInv
-        {rep : Type} (repInv : Ensemble rep)
-        {mutIdx : Type}
-  : forall (muts muts' : mutIdx -> mutatorMethodType rep),
-      mutatorInv repInv muts ->
-      pointwise_relation mutIdx (refineMutator repInv (@Return _)) muts muts'->
-      mutatorInv repInv muts'.
-  Proof.
-    simpl; unfold pointwise_relation; intros; eapply_hyp; eauto.
-    generalize (H0 idx _ n H1).
-    setoid_rewrite refine_refine; autorewrite with refine_monad; try reflexivity; eauto.
-  Qed.
-
-  Hint Resolve refineMutatorInv.
-
-  (* The [refineADT_Build_ADT_Mutators lemma shows that refining mutators
-   is a valid ADT refinement; the statement hews closely to the standard
-   Parametric Morphism declaration style for future compatibility (hopefully). *)
-
-  Lemma refineADT_Build_ADT_Mutators rep (repInv : Ensemble rep) mutIdx obsIdx obs :
-    (respectful_hetero
-       _ _ (fun x => mutatorInv repInv x -> ADT) (fun x => mutatorInv _ x -> ADT)
-       (pointwise_relation mutIdx (@refineMutator rep rep repInv (@Return _)))
-       (fun x y mInv mInv' => forall mI mI', refineADT (mInv mI) (mInv' mI')))
-      (fun mut => @Build_ADT rep repInv mutIdx obsIdx mut obs) (fun mut => @Build_ADT rep repInv mutIdx obsIdx mut obs).
-  Proof.
-    unfold respectful_hetero; intros.
-    let A := match goal with |- refineADT ?A ?B => constr:(A) end in
-    let B := match goal with |- refineADT ?A ?B => constr:(B) end in
-    eapply (@refinesADT A B (@Return _) id id);
-      unfold id, pointwise_relation in *; simpl in *; intros;
-      [ auto
-      | autorewrite with refine_monad; reflexivity
-      | inversion_by computes_to_inv; subst; eauto].
-  Qed.
-
-  (* [BD: I'm registering the above as a proper relation on the off-chance that the
-   setoid machinary can take advantage of it :) ]*)
-  Instance refineADT_Build_ADT_Mutators_Proper rep (repInv : Ensemble rep) mutIdx obsIdx obs :
-    Proper
-      (respectful_hetero
-         _ _ (fun x => mutatorInv repInv x -> ADT) (fun x => mutatorInv _ x -> ADT)
-         (pointwise_relation mutIdx (@refineMutator rep rep repInv (@Return _)))
-         (fun x y mInv mInv' => forall mI mI', refineADT (mInv mI) (mInv' mI')))
-      (fun mut => @Build_ADT rep repInv mutIdx obsIdx mut obs).
-  Proof.
-    apply refineADT_Build_ADT_Mutators.
-  Qed.
-
-  (* If the proof of [MutatorMethodsInv] doesn't depend on [MutatorMethods]
-   there's no problem using the existing Parametric Morphism machinery.
-   (Of course, this means that repInv is trivial.) *)
-
-  Add Parametric Morphism rep repInv mutIdx obsIdx mutInv
-  : (fun ms os => @Build_ADT rep repInv mutIdx obsIdx ms os (mutInv ms))
-      with signature
-      (pointwise_relation _ (@refineMutator _ _ repInv (@Return _)))
-        ==> (pointwise_relation _ (@refineObserver _ _ repInv (@Return _)))
-        ==> refineADT
-        as refineADT_Build_ADT_Mutators'.
-  Proof.
-    intros.
-    let A := match goal with |- refineADT ?A ?B => constr:(A) end in
-    let B := match goal with |- refineADT ?A ?B => constr:(B) end in
-    eapply (@refinesADT A B (@Return _) id id);
-      unfold id, pointwise_relation in *; simpl in *; intros;
-      auto; inversion_by computes_to_inv; subst; eauto.
-  Qed.
-
-  (* Refining observers and mutators at the same time is also a valid
-   refinement. [BD: I've come to the conclusion that smaller refinement
-   steps are better, so using the previous refinements should be the
-   preferred mode. ]*)
-
-  Lemma refineADT_Build_ADT_Both rep (repInv : Ensemble rep) mutIdx obsIdx :
-    (respectful_hetero
-       _ _ _ _
-       (pointwise_relation mutIdx (@refineMutator rep rep repInv (@Return _)))
-       (fun x y => respectful_hetero
-                     _ _ (fun _ => mutatorInv repInv x -> ADT) (fun _ => mutatorInv _ y -> ADT)
-                     (pointwise_relation obsIdx (@refineObserver rep rep repInv (@Return _)))
-                     (fun obs obs' mInv mInv' =>
-                        forall mI mI', refineADT (mInv mI) (mInv' mI'))))
-      (@Build_ADT rep repInv mutIdx obsIdx) (@Build_ADT rep repInv mutIdx obsIdx).
-  Proof.
-    unfold respectful_hetero; intros.
-    rewrite refineADT_Build_ADT_Observer; eauto.
-    eapply refineADT_Build_ADT_Mutators; eauto.
-  Qed.
-
-  (** If we had dependent setoid relations in [Type], then we could write
+   If we had dependent setoid relations in [Type], then we could write
 
 <<
 Add Parametric Morphism : @Build_ADT
@@ -368,7 +230,90 @@ Qed.
 
     But, alas, Matthieu is still working on those.  So the rewrite
     machinery won't work very well when we're switching reps, and
-    we'll instead have to use [etransitivity] and [apply] things. *)
+    we'll instead have to use [etransitivity] and [apply] the
+    [refineADT_Build_ADT_Rep] lemma to switch representations.
+
+    The statement of [refineADT_Build_ADT_Rep] mimics the notation for
+    registering [Parametric Morphism]s so that it will be easy to
+    integrate if dependent setoid relations are added.
+
+ **)
+
+  Lemma refineADT_Build_ADT_Rep oldRep newRep
+        (BiR : oldRep -> newRep -> Prop)
+        mutIdx obsIdx :
+    (respectful_hetero
+       (mutIdx -> mutatorMethodType oldRep)
+       (mutIdx -> mutatorMethodType newRep)
+       (fun oldMuts => (obsIdx -> observerMethodType oldRep) -> ADT)
+       (fun newMuts => (obsIdx -> observerMethodType newRep) -> ADT)
+       (fun oldMuts newMuts =>
+          forall mutIdx,
+            @refineMutator oldRep newRep BiR
+                           (oldMuts mutIdx)
+                           (newMuts mutIdx))
+       (fun x y => respectful_hetero
+                     (obsIdx -> observerMethodType oldRep)
+                     (obsIdx -> observerMethodType newRep)
+                     (fun _ => ADT)
+                     (fun _ => ADT)
+                     (fun obs obs' =>
+                        forall obsIdx,
+                          @refineObserver oldRep newRep BiR
+                                         (obs obsIdx)
+                                         (obs' obsIdx))
+                     (fun obs obs' => refineADT)))
+      (@Build_ADT oldRep mutIdx obsIdx)
+      (@Build_ADT newRep mutIdx obsIdx).
+  Proof.
+    unfold Proper, respectful_hetero; intros.
+    let A := match goal with |- refineADT ?A ?B => constr:(A) end in
+    let B := match goal with |- refineADT ?A ?B => constr:(B) end in
+    eapply (@refinesADT A B BiR id id);
+      unfold id, pointwise_relation in *; simpl in *; intros; eauto.
+  Qed.
+
+  (* Thankfully, we can register a number of different refinements
+     which follow from [refineADT_Build_ADT_Rep] as [Parametric Morphism]s.*)
+
+  (* Refining Observers is a valid ADT refinement. *)
+  Add Parametric Morphism rep mutIdx obsIdx ms
+  : (fun os => @Build_ADT rep mutIdx obsIdx ms os)
+      with signature
+      (pointwise_relation _ (@refineObserver _ _ eq))
+        ==> refineADT
+        as refineADT_Build_ADT_Observer.
+  Proof.
+    intros; eapply refineADT_Build_ADT_Rep; eauto; reflexivity.
+  Qed.
+
+  (* Refining Mutators is also a valid ADT refinement. *)
+
+  Add Parametric Morphism rep mutIdx obsIdx obs
+  : (fun ms => @Build_ADT rep mutIdx obsIdx ms obs)
+      with signature
+      (pointwise_relation _ (@refineMutator _ _ eq))
+        ==> refineADT
+        as refineADT_Build_ADT_Mutators.
+  Proof.
+    intros; eapply refineADT_Build_ADT_Rep; eauto; reflexivity.
+  Qed.
+
+  (* Refining observers and mutators at the same time is also a valid
+   refinement. [BD: I've come to the conclusion that smaller refinement
+   steps are better, so using the previous refinements should be the
+   preferred mode. ]*)
+
+  Add Parametric Morphism rep mutIdx obsIdx
+  : (fun ms os => @Build_ADT rep mutIdx obsIdx ms os)
+      with signature
+      (pointwise_relation _ (@refineMutator _ _ eq))
+        ==> (pointwise_relation _ (@refineObserver _ _ eq))
+        ==> refineADT
+        as refineADT_Build_ADT_Both.
+  Proof.
+    intros; eapply refineADT_Build_ADT_Rep; eauto; reflexivity.
+  Qed.
 
 (* Given an abstraction function, we can transform the rep of a pickImpl ADT. *)
 
@@ -383,152 +328,143 @@ Qed.
                  (fun idx nm n nm' => MutatorSpec idx (abs nm) n (abs nm'))
                  (fun idx nm => ObserverSpec idx (abs nm))).
   Proof.
-    econstructor 1 with (abs := fun nm => Return (abs nm))
+    econstructor 1 with (BiR := fun om nm => om = (abs nm))
                           (mutatorMap := @id MutatorIndex)
                           (observerMap := @id ObserverIndex);
-    compute; intros; inversion_by computes_to_inv; subst; eauto.
-  Qed.
-
-  (* The weakest reasonable invariant on a new representation is that
-     the abstraction of a member satisfies the old invariant. *)
-  Definition abs_repInv {newRep oldRep : Type}
-             (abs : newRep -> Comp oldRep)
-             (repInv : Ensemble oldRep) (nr : newRep) :=
-    computational_inv repInv (abs nr).
-
-  Arguments abs_repInv newRep oldRep abs repInv nr / .
-
-  (* Refining the representation type is a valid refinement,
-     as long as the new methods are valid refinements and the
-     updated the old invariant is preserved by abstraction. *)
-
-  Lemma refineADT_Build_ADT_Rep oldRep newRep
-        (abs : newRep -> Comp oldRep)
-        (oldRepInv : Ensemble oldRep)
-        (newRepInv : Ensemble newRep)
-        (absSafe : forall nr, newRepInv nr ->
-                              computational_inv oldRepInv (abs nr))
-        mutIdx obsIdx :
-    (respectful_hetero
-       (mutIdx -> mutatorMethodType oldRep)
-       (mutIdx -> mutatorMethodType newRep)
-       (fun oldMuts => (obsIdx -> observerMethodType oldRep) ->
-                 mutatorInv oldRepInv oldMuts -> ADT)
-       (fun newMuts => (obsIdx -> observerMethodType newRep) ->
-                    mutatorInv (newRepInv) newMuts -> ADT)
-       (fun oldMuts newMuts =>
-          forall mutIdx,
-            @refineMutator oldRep newRep (newRepInv) abs
-                           (oldMuts mutIdx)
-                           (newMuts mutIdx))
-       (fun x y => respectful_hetero
-                     (obsIdx -> observerMethodType oldRep)
-                     (obsIdx -> observerMethodType newRep)
-                     (fun _ => mutatorInv oldRepInv x -> ADT)
-                     (fun _ => mutatorInv _ y -> ADT)
-                     (fun obs obs' =>
-                        forall obsIdx,
-                          @refineObserver oldRep newRep (newRepInv) abs
-                                         (obs obsIdx)
-                                         (obs' obsIdx))
-                     (fun obs obs' mInv mInv' =>
-                        forall mI mI', refineADT (mInv mI) (mInv' mI'))))
-      (@Build_ADT oldRep oldRepInv mutIdx obsIdx)
-      (@Build_ADT newRep newRepInv mutIdx obsIdx).
-  Proof.
-    unfold Proper, respectful_hetero; intros.
-    let A := match goal with |- refineADT ?A ?B => constr:(A) end in
-    let B := match goal with |- refineADT ?A ?B => constr:(B) end in
-    eapply (@refinesADT A B abs id id);
-      unfold id, pointwise_relation in *; simpl in *; intros; eauto.
+    compute; intros;
+    [inversion_by computes_to_inv; subst; eauto
+     | inversion_by computes_to_inv; subst; eauto].
   Qed.
 
   (* We can always build a default implementation (computation?) for the
      mutators of an ADT with an updated representation using the old
      mutators. *)
   Definition absMutatorMethods oldRep newRep
-        (abs : newRep -> Comp oldRep)
+        (BiR : oldRep -> newRep -> Prop)
         mutIdx
         (oldMuts : mutIdx -> mutatorMethodType oldRep) idx nr n : Comp newRep :=
-    (or' <- abs nr;
-    {nm | refine (oldMuts idx or' n) (abs nm)})%comp.
+    {nr' | forall or,
+             BiR or nr ->
+             exists or',
+               (oldMuts idx or n) ↝ or' /\
+               BiR or' nr'}%comp.
 
   Lemma refine_absMutatorMethods oldRep newRep
-        newRepInv
-        (abs : newRep -> Comp oldRep)
+        (BiR : oldRep -> newRep -> Prop)
         mutIdx
         (oldMuts : mutIdx -> mutatorMethodType oldRep)
   : forall idx,
-      @refineMutator oldRep newRep newRepInv abs
+      @refineMutator oldRep newRep BiR
                      (oldMuts idx)
-                     (absMutatorMethods abs oldMuts idx).
+                     (absMutatorMethods BiR oldMuts idx).
   Proof.
     unfold refineMutator, absMutatorMethods, refine; intros.
-    inversion_by computes_to_inv; econstructor; eauto.
+    inversion_by computes_to_inv.
+    destruct (H0 _ H) as [or' [Comp_or BiR_or''] ].
+    econstructor; eauto.
   Qed.
 
   (* Always unfold absMutatorMethods. *)
-  Global Arguments absMutatorMethods oldRep newRep abs mutIdx oldMuts / idx nr n.
+  Global Arguments absMutatorMethods oldRep newRep BiR mutIdx oldMuts / idx nr n.
 
   Hint Resolve refine_absMutatorMethods.
-
-  Lemma absMutatorMethodsInv
-        oldRep newRep
-        (abs : newRep -> Comp oldRep)
-        (oldRepInv : Ensemble oldRep)
-        mutIdx
-        (oldMuts : mutIdx -> mutatorMethodType oldRep)
-  : mutatorInv oldRepInv oldMuts ->
-    mutatorInv (abs_repInv abs oldRepInv) (absMutatorMethods abs oldMuts).
-  Proof.
-    unfold absMutatorMethods, abs_repInv; simpl in *; intros;
-    inversion_by computes_to_inv; eauto.
-  Qed.
 
   (* A similar approach works for observers. *)
 
   Definition absObserverMethods oldRep newRep
-        (abs : newRep -> Comp oldRep)
-        obsIdx
-        (oldObs : obsIdx -> observerMethodType oldRep) idx nr n : Comp nat :=
-    (or' <- abs nr;
-    {n' | refine (oldObs idx or' n) (ret n')})%comp.
+             (BiR : oldRep -> newRep -> Prop)
+             obsIdx
+             (oldObs : obsIdx -> observerMethodType oldRep) idx nr n : Comp nat :=
+    {n' | forall or,
+            BiR or nr ->
+            (oldObs idx or n) ↝ n'}%comp.
 
   Lemma refine_absObserverMethods oldRep newRep
-        newRepInv
-        (abs : newRep -> Comp oldRep)
+        (BiR : oldRep -> newRep -> Prop)
         obsIdx
         (oldObs : obsIdx -> observerMethodType oldRep)
   : forall idx,
-      @refineObserver oldRep newRep newRepInv abs
-                     (oldObs idx)
-                     (absObserverMethods abs oldObs idx).
+      @refineObserver oldRep newRep BiR (oldObs idx)
+                     (absObserverMethods BiR oldObs idx).
   Proof.
     unfold refineObserver, absObserverMethods, refine; intros.
-    inversion_by computes_to_inv; econstructor; eauto.
+    inversion_by computes_to_inv; eauto.
   Qed.
 
-  Global Arguments absObserverMethods oldRep newRep abs obsIdx oldObs / idx nr n .
-
+  Global Arguments absObserverMethods oldRep newRep BiR obsIdx oldObs / idx nr n .
 
   Hint Resolve refine_absObserverMethods.
 
-  (* We can refine an ADT using the above default mutator / observer / invariant
+  (* We can refine an ADT using the above default mutator and observer
      implementations. *)
 
   Lemma refineADT_Build_ADT_Rep_default oldRep newRep
-        (abs : newRep -> Comp oldRep)
-        (oldRepInv : Ensemble oldRep)
-        mutIdx obsIdx oldMuts oldObs oldInv :
+        (BiR : oldRep -> newRep -> Prop)
+        mutIdx obsIdx oldMuts oldObs :
     refineADT
-      (@Build_ADT oldRep oldRepInv mutIdx obsIdx oldMuts oldObs oldInv)
-      (@Build_ADT newRep (abs_repInv abs oldRepInv) mutIdx obsIdx
-                  (absMutatorMethods abs oldMuts)
-                  (absObserverMethods abs oldObs)
-                  (absMutatorMethodsInv oldInv)).
+      (@Build_ADT oldRep mutIdx obsIdx oldMuts oldObs)
+      (@Build_ADT newRep mutIdx obsIdx
+                  (absMutatorMethods BiR oldMuts)
+                  (absObserverMethods BiR oldObs)).
   Proof.
     eapply refineADT_Build_ADT_Rep; eauto.
   Qed.
+
+  Section SimplifyRep.
+
+  (* If a representation has extraneous information (perhaps intermediate
+     data introduced during refinement), simplifying the representation
+     is a valid refinement. *)
+
+    Variable oldRep : Type.
+    Variable newRep : Type.
+
+    Variable simplifyf : oldRep -> newRep.
+    Variable concretize : newRep -> oldRep.
+    Variable BiR : oldRep -> newRep -> Prop.
+
+    Notation "ro ≃ rn" := (BiR ro rn) (at level 70).
+
+    Definition simplifyMutatorMethods
+               mutIdx (oldMuts : mutIdx -> mutatorMethodType oldRep)
+               idx r_n n : Comp newRep :=
+      (r_o' <- (oldMuts idx (concretize r_n) n);
+       ret (simplifyf r_o'))%comp.
+
+  Definition simplifyObserverMethods
+             obsIdx (oldObs : obsIdx -> observerMethodType oldRep)
+             idx nr n : Comp nat :=
+    oldObs idx (concretize nr) n.
+
+  Definition simplifyRep
+             mutIdx obsIdx oldMuts oldObs :
+    (forall r_n r_o,
+                (r_o ≃ r_n) ->
+                forall idx n,
+                  refineEquiv (r_o'' <- oldMuts idx r_o n;
+                              {r_n' | r_o'' ≃ r_n'})
+                              (r_o'' <- oldMuts idx (concretize r_n) n;
+                              ret (simplifyf r_o''))) ->
+    (forall r_n r_o,
+                (r_o ≃ r_n) ->
+                forall idx n,
+                  refineEquiv (oldObs idx r_o n)
+                              (oldObs idx (concretize r_n) n)) ->
+    refineADT
+      (@Build_ADT oldRep mutIdx obsIdx oldMuts oldObs)
+      (@Build_ADT newRep mutIdx obsIdx
+                  (simplifyMutatorMethods oldMuts)
+                  (simplifyObserverMethods oldObs)).
+  Proof.
+    econstructor 1 with
+    (BiR := BiR)
+      (mutatorMap := @id mutIdx)
+      (observerMap := @id obsIdx); simpl; eauto.
+    - unfold simplifyMutatorMethods; intros; eapply H; eauto.
+    - unfold simplifyObserverMethods; intros; eapply H0; eauto.
+  Qed.
+
+  End SimplifyRep.
 
 (** TODO: Update this to reflect the new definition of ADT + ADT
     Refinement *)
@@ -573,44 +509,41 @@ Qed.
 
 Hint Rewrite refine_pick_refine : refine_monad.
 
-  (* Honing tactic for refining the mutator method with the specified index.
-     This version of the tactic develops the new mutator body interactively. *)
-  Tactic Notation "hone" "mutator" constr(mutIdx) :=
-    let A := match goal with |- Sharpened ?A => constr:(A) end in
-    let mutIdx_eq' := fresh in
-    let Rep' := eval simpl in (Rep A) in
-    let RepInv' := eval simpl in (RepInv A) in
+(* Honing tactic for refining the observer method with the specified index.
+     This version of the tactic takes the new implementation as an argument. *)
+Tactic Notation "hone" "observer" constr(obsIdx) "using" constr(obsBody) :=
+  let A :=
+      match goal with
+          |- Sharpened ?A => constr:(A) end in
+  let mutIdx_eq' := fresh in
+  let Rep' := eval simpl in (Rep A) in
     let MutatorIndex' := eval simpl in (MutatorIndex A) in
     let ObserverIndex' := eval simpl in (ObserverIndex A) in
     let MutatorMethods' := eval simpl in (MutatorMethods A) in
     let ObserverMethods' := eval simpl in (ObserverMethods A) in
-    let MutatorMethodsInv' := eval simpl in (MutatorMethodsInv A) in
-    assert (forall idx idx' : MutatorIndex', {idx = idx'} + {idx <> idx'})
-      as mutIdx_eq' by (decide equality);
+      assert (forall idx idx' : ObserverIndex', {idx = idx'} + {idx <> idx'})
+        as obsIdx_eq' by (decide equality);
       let RefineH := fresh in
-      assert ({mutBody | pointwise_relation _ (refineMutator RepInv' (@Return Rep'))
-                                 MutatorMethods'
-                                 (fun idx => if (mutIdx_eq' idx mutIdx) then
-                                               mutBody
+      assert (pointwise_relation ObserverIndex' (refineObserver (@eq Rep'))
+                                 (ObserverMethods')
+                                 (fun idx => if (obsIdx_eq' idx ()) then
+                                               obsBody
                                              else
-                                               MutatorMethods' idx)}) as RefineH;
-        [eexists _; let mutIdx' := fresh in
-         unfold pointwise_relation; intro mutIdx';
-         destruct (mutIdx_eq' mutIdx' mutIdx); simpl; intros; autorewrite with refine_monad; simpl;
+                                               ObserverMethods' idx)) as RefineH;
+        [let obsIdx' := fresh in
+         unfold pointwise_relation; intro obsIdx';
+         destruct (obsIdx_eq' obsIdx' ()); simpl; intros; simpl;
          [idtac | (* Replaced mutator case left to user*)
-          reflexivity] (* Otherwise, they are the same *)
+          subst; reflexivity] (* Otherwise, they are the same *)
         | eapply SharpenStep;
-          [eapply (@refineADT_Build_ADT_Mutators
-                         Rep' RepInv' MutatorIndex' ObserverIndex'
-                         ObserverMethods'
+          [eapply (@refineADT_Build_ADT_Observer
+                         Rep' ObserverIndex' MutatorIndex'
                          MutatorMethods'
-                         (fun idx => if (mutIdx_eq' idx ()) then
-                                       (proj1_sig RefineH)
+                         ObserverMethods'
+                         (fun idx => if (obsIdx_eq' idx ()) then
+                                       obsBody
                                      else
-                                       MutatorMethods' idx) (proj2_sig RefineH)
-                         MutatorMethodsInv'
-                         (refineMutatorInv MutatorMethodsInv' (proj2_sig RefineH))
-                      ); simpl
+                                       ObserverMethods' idx) RefineH)
           | idtac] ]; cbv beta in *; simpl in *.
 
   (* Honing tactic for refining the mutator method with the specified index.
@@ -621,16 +554,14 @@ Hint Rewrite refine_pick_refine : refine_monad.
             |- Sharpened ?A => constr:(A) end in
     let mutIdx_eq' := fresh in
     let Rep' := eval simpl in (Rep A) in
-    let RepInv' := eval simpl in (RepInv A) in
     let MutatorIndex' := eval simpl in (MutatorIndex A) in
     let ObserverIndex' := eval simpl in (ObserverIndex A) in
     let MutatorMethods' := eval simpl in (MutatorMethods A) in
     let ObserverMethods' := eval simpl in (ObserverMethods A) in
-    let MutatorMethodsInv' := eval simpl in (MutatorMethodsInv A) in
       assert (forall idx idx' : MutatorIndex', {idx = idx'} + {idx <> idx'})
         as mutIdx_eq' by (decide equality);
       let RefineH := fresh in
-      assert (pointwise_relation MutatorIndex' (refineMutator RepInv' (@Return Rep'))
+      assert (pointwise_relation MutatorIndex' (refineMutator (@eq Rep'))
                                  (MutatorMethods')
                                  (fun idx => if (mutIdx_eq' idx ()) then
                                                mutBody
@@ -638,25 +569,23 @@ Hint Rewrite refine_pick_refine : refine_monad.
                                                MutatorMethods' idx)) as RefineH;
         [let mutIdx' := fresh in
          unfold pointwise_relation; intro mutIdx';
-         destruct (mutIdx_eq' mutIdx' ()); simpl; intros; autorewrite with refine_monad; simpl;
+         destruct (mutIdx_eq' mutIdx' ()); simpl; intros;
+         setoid_rewrite refineEquiv_pick_eq'; autorewrite with refine_monad; simpl;
          [idtac | (* Replaced mutator case left to user*)
-          reflexivity] (* Otherwise, they are the same *)
+          subst; reflexivity] (* Otherwise, they are the same *)
         | eapply SharpenStep;
           [eapply (@refineADT_Build_ADT_Mutators
-                         Rep' RepInv' ObserverIndex' MutatorIndex'
+                         Rep' ObserverIndex' MutatorIndex'
                          ObserverMethods'
                          MutatorMethods'
                          (fun idx => if (mutIdx_eq' idx ()) then
                                        mutBody
                                      else
-                                       MutatorMethods' idx) RefineH
-                         MutatorMethodsInv'
-                         (refineMutatorInv MutatorMethodsInv' RefineH)
-                      ); simpl
+                                       MutatorMethods' idx) RefineH)
           | idtac] ]; cbv beta in *; simpl in *.
 
 (* Honing tactic for refining the ADT representation which provides
    default observer and mutator implementations. *)
-Tactic Notation "hone" "representation" "using" constr(absf) :=
+Tactic Notation "hone" "representation" "using" constr(BiSR) :=
     eapply SharpenStep;
-    [eapply refineADT_Build_ADT_Rep_default with (abs := absf) | idtac].
+    [eapply refineADT_Build_ADT_Rep_default with (BiR := BiSR) | idtac].
