ADT.v
@@ -17,22 +17,11 @@ Definition observerMethodType (Ty : Type) :=
   -> nat (* Actual argument*)
   -> Comp nat. (* Return value *)
 
-(** Correctness property for mutators: Mutators should maintain
-   representation invariants. **)
-Definition mutatorInv rep (repInv : Ensemble rep) mutIdx mutators :=
-  forall (idx : mutIdx) (r : rep) (n : nat),
-    repInv r -> computational_inv repInv (mutators idx r n).
-
-Arguments mutatorInv rep repInv mutIdx mutators /.
-
 (** Interface of an ADT *)
 Record ADT :=
   {
     Rep : Type;
     (** The way we model state mathematically *)
-
-    RepInv : Rep -> Prop;
-    (** Invariants on the Representation **)
 
     MutatorIndex : Type;
     (** The index set of mutators *)
@@ -43,13 +32,7 @@ Record ADT :=
     MutatorMethods : MutatorIndex -> mutatorMethodType Rep;
     (** Mutator method implementations *)
 
-    ObserverMethods : ObserverIndex -> observerMethodType Rep;
+    ObserverMethods : ObserverIndex -> observerMethodType Rep
     (** Observer method implementations *)
-
-    MutatorMethodsInv : mutatorInv RepInv MutatorMethods
-    (** Mutator methods maintain Representation Invariants **)
-
-    (** We probably want some sort of observer method specs as well.
-     That can wait until the next iteration of the ADT with arbitrary signatures. **)
 
   }.
